Modifs Partie 3

Krivine.ml
@@ -1,0 +1,24 @@
+type Variable;;
+type instruction = Access of int| Grab |Push of code;;
+type code == instruction list;;(*instruction list*)
+(*type environment = V of Variable|E of (code*environment) list;;*)
+type stack == (code*environment) list;;(*code*environment list*)
+type environment == stack;;
+type state = {mutable c:code;mutable e:environment;mutable s:stack};;
+
+
+let rec execute st =
+if st.c=[] then st else
+match hd(st.c) with
+|Access 0->execute {c=fst(hd(st.e));e=snd(hd(st.e));s=st.s};
+|Access n->st.c=Access (n-1)::tl(st.c);st.e=tl(st.e);execute st;
+|Grab->st.c=tl(st.c);st.e=hd(st.s)::st.e;st.s=tl(st.s);execute st;
+|Push cc->st.s=(cc,st.e)::st.s;st.c=tl(st.c);execute st;;
+
+let rec execute st =
+if st.c=[] then st else
+match hd(st.c) with
+|Access 0->st.c=fst(hd(st.e));st.e=snd(hd(st.e));execute st;
+|Access n->st.c=Access (n-1)::tl(st.c);st.e=tl(st.e);execute st;
+|Grab->st.c=tl(st.c);st.e=hd(st.s)::st.e;st.s=tl(st.s);execute st;
+|Push cc->st.s=(cc,st.e)::st.s;st.c=tl(st.c);execute st;;
